CPPSynth/Generate.v
@@ -1,4 +1,4 @@
-Require Import 
+Require Import
   Coq.Arith.Compare_dec
   Coq.Numbers.DecimalString
   Coq.Numbers.DecimalNat
@@ -9,6 +9,7 @@ Require Import
   CPPSynth.Exception
   CPPSynth.Gallina
   CPPSynth.CPPAst
+  CPPSynth.CPPAstTrans
   CPPSynth.Monad.
 
 Module cg.
@@ -16,7 +17,7 @@ Module cg.
     typeexpr_id (idexpr_id scope_none s).
   Definition shared_ptr_of (type : typeexpr_t) : typeexpr_t :=
   typeexpr_id (
-    idexpr_template (scope_id "std" scope_none) (templateid "shared_ptr"
+    idexpr_template (scope_id "std" scope_none) (templateid_make "shared_ptr"
       (tplargs_cons (tplarg_type type) tplargs_nil))).
   Definition constref_of (type : typeexpr_t) : typeexpr_t :=
     typeexpr_reference (typeexpr_const type).
@@ -25,7 +26,7 @@ Module cg.
   Definition declval_of (type : typeexpr_t) :=
     expr_call
       (expr_id (
-        idexpr_template (scope_id "std" scope_none) (templateid "declval"
+        idexpr_template (scope_id "std" scope_none) (templateid_make "declval"
           (tplargs_cons (tplarg_type type) tplargs_nil))))
       callargs_nil.
   Definition move_of (expr : expr_t) : expr_t :=
@@ -35,7 +36,7 @@ Module cg.
   Definition make_shared_of (type : typeexpr_t) (args : list expr_t) :=
     expr_call
       (expr_id (
-        idexpr_template (scope_id "std" scope_none) (templateid "make_shared"
+        idexpr_template (scope_id "std" scope_none) (templateid_make "make_shared"
           (tplargs_cons (tplarg_type type) tplargs_nil))))
       (make_callargs args).
   Definition fn_type (result_type : typeexpr_t) (args : list (option string * typeexpr_t)) : typeexpr_t :=
@@ -44,7 +45,7 @@ Module cg.
         | None => funarg_anon type
         | Some n => funarg_named type n
       end) args) in
-    typeexpr_function (funtypeexpr result_type fnargs false).
+    typeexpr_function (funtypeexpr_make result_type fnargs fnqual.none false).
   Definition type_auto := typeexpr_primitive primtype.auto.
   Definition throw_logic_error (msg : string) :=
     let std_logic_error :=
@@ -52,12 +53,13 @@ Module cg.
     let arg := expr_literal (literal.str msg) in
     expr_throw (expr_call std_logic_error (make_callargs (arg :: nil))).
   Definition deleted_constructor (name : string) (args : list funarg_t): decl_t :=
-    decl_consdesdef_special
-      nil
+    decl_consdesdef
+      declspec.none
       (idexpr_id scope_none name)
       (make_funargs args)
-      nil
-      special_fundef.def_delete.
+      fnqual.none
+      attrspec.none
+      funbody_delete.
 End cg.
 
 Fixpoint make_tplargs (args : list tplarg_t) : tplargs_t :=
@@ -89,7 +91,7 @@ Module env.
     match fn with
       | expr.global n =>
         let tplargs := make_tplargs (map (fun arg => tplarg_type arg) args) in
-        typeexpr_id (idexpr_template scope_none (templateid n tplargs))
+        typeexpr_id (idexpr_template scope_none (templateid_make n tplargs))
       | expr.app fn arg =>
         to_type_template_apply fn (args ++ (to_type arg this) :: nil) this
       | _ => typeexpr_primitive (primtype.auto)
@@ -123,7 +125,7 @@ End env.
 
 Definition product_unfold (e : expr.t) : list (option string * expr.t) * expr.t :=
   let head := nil in
-  (fix loop (e : expr.t) (head : list (option string * expr.t)) 
+  (fix loop (e : expr.t) (head : list (option string * expr.t))
       : list (option string * expr.t) * expr.t :=
     match e with
       | expr.product argname argtype body =>
@@ -137,7 +139,7 @@ Definition product_unfold (e : expr.t) : list (option string * expr.t) * expr.t 
 Definition product_named_unfold (e : expr.t) : list (string * expr.t) * expr.t :=
   let head := nil in
   let index := 0 in
-  (fix loop (e : expr.t) (index : nat) (head : list (string * expr.t)) 
+  (fix loop (e : expr.t) (index : nat) (head : list (string * expr.t))
       : list (string * expr.t) * expr.t :=
     match e with
       | expr.product argname argtype body =>
@@ -182,25 +184,40 @@ Definition inductive_fwd (i : inductive.t) : list decl_t :=
   map (one_inductive_fwd) ois.
 
 Definition gen_virtual_destructor_decldef (name : string) : decl_t :=
+  let ds := declspec.none in
+  let ds := declspec.set_virtual ds in
   decl_consdesdef
-    (decl_specifier.ds_virtual :: nil)
+    ds
     (idexpr_destructor scope_none name)
     (make_funargs nil)
-    nil
-    ctor_initializers_nil
-    (make_stmts nil).
+    fnqual.none
+    attrspec.none
+    (funbody_stmts cinits_nil (make_stmts nil)).
 
 Definition make_repr_base_class (name : string) :=
-  decl_class 
-    (idexpr_id scope_none name) 
-    false 
+  let repr_cls_type := typeexpr_id (idexpr_id scope_none name) in
+  let eq_operator :=
+    decl_fundef
+      (declspec.set_virtual declspec.none)
+      (funtypeexpr_make
+        (typeexpr_primitive primtype.bool)
+        (make_funargs (funarg_named (cg.constref_of repr_cls_type) "other" :: nil))
+        (fnqual.set_noexcept (fnqual.set_const fnqual.none))
+        false)
+      (idexpr_operator scope_none (overloadable_operator.binary binop.eq))
+      attrspec.none
+      funbody_abstract in
+  decl_class
+    (idexpr_id scope_none name)
+    false
     clsinherits_nil
     (clsdecls_cons
       (clsdecl_group
         visibility_spec.vis_public
-        (decls_cons
-          (gen_virtual_destructor_decldef name)
-          decls_nil))
+        (make_decls
+          (gen_virtual_destructor_decldef name ::
+          eq_operator ::
+          nil)))
       clsdecls_nil).
 
 Definition constructor_reprclass_name (cons : inductive_constructor.t) : string :=
@@ -210,11 +227,11 @@ Definition constructor_reprclass_members (cons : inductive_constructor.t)
     : list (string * expr.t) :=
   fst (product_named_unfold (inductive_constructor.type cons)).
 
-Fixpoint make_ctor_initializers (is : list ctor_initializer_t)
-    : ctor_initializers_t :=
+Fixpoint make_cinits (is : list cinit_t)
+    : cinits_t :=
   match is with
-    | nil => ctor_initializers_nil
-    | cons i is => ctor_initializers_cons i (make_ctor_initializers is)
+    | nil => cinits_nil
+    | cons i is => cinits_cons i (make_cinits is)
   end.
 
 Definition make_constructor_repr_class
@@ -222,11 +239,19 @@ Definition make_constructor_repr_class
     (environ : env.t) :=
   let name := constructor_reprclass_name cons in
   let members := constructor_reprclass_members cons in
+
+  let repr_cls_id := idexpr_id scope_none name in
+  let repr_cls_type := typeexpr_id repr_cls_id in
+  let repr_constptr := typeexpr_pointer (typeexpr_const repr_cls_type) in
+
+  let base_cls_id := (idexpr_id scope_none "repr_base") in
+  let base_cls_type := typeexpr_id base_cls_id in
+
   let member_decls := map
     (fun (mem : string * expr.t) =>
       let (name, e) := mem in
       let type := env.to_type e environ in
-      decl_simple nil type (idexpr_id scope_none name) nil) members in
+      decl_simple declspec.none type (idexpr_id scope_none name) attrspec.none) members in
   let init_formal_args := map
     (fun (mem : string * expr.t) =>
       let (name, e) := mem in
@@ -235,26 +260,73 @@ Definition make_constructor_repr_class
   let initializers := map
     (fun (mem : string * expr.t) =>
       let (name, e) := mem in
-      ctor_initializer 
+      cinit_make
         (idexpr_id scope_none name)
         (cg.move_of (expr_id (idexpr_id scope_none (name ++ "_init"))))) members in
   let cls_constructor := decl_consdesdef
-    nil
+    declspec.none
     (idexpr_id scope_none name)
     (make_funargs init_formal_args)
-    nil
-    (make_ctor_initializers initializers)
-    stmts_nil in
-  let eq_operator :=
+    fnqual.none
+    attrspec.none
+    (funbody_stmts
+      (make_cinits initializers)
+      stmts_nil) in
+  let overridden_eq_operator :=
     decl_fundef
-  decl_class 
-    (idexpr_id scope_none (name))
+      declspec.none
+      (funtypeexpr_make
+        (typeexpr_primitive primtype.bool)
+        (make_funargs (funarg_named (cg.constref_of base_cls_type) "other" :: nil))
+        (fnqual.set_noexcept (fnqual.set_const fnqual.none))
+        false)
+      (idexpr_operator scope_none (overloadable_operator.binary binop.eq))
+      (attrspec.set_override attrspec.none)
+      (funbody_stmts cinits_nil
+        (make_stmts
+          (stmt_ifelse
+            (condition_decl
+              declspec.none (typeexpr_primitive primtype.auto)
+              (idexpr_id scope_none "spec")
+              attrspec.none
+              (expr_dynamic_cast repr_constptr (expr_unop unop.address_of (expr_id (idexpr_id scope_none "other")))))
+            (stmt_block (make_stmts
+              (stmt_return (expr_binop binop.eq
+                (expr_unop unop.deref (expr_id (idexpr_id scope_none "this")))
+                (expr_unop unop.deref (expr_id (idexpr_id scope_none "spec"))))
+              :: nil)))
+            (stmt_block (make_stmts
+              (stmt_return (expr_id (idexpr_id scope_none "false")) :: nil))) ::
+          nil))) in
+  let member_compare := map
+    (fun (mem : string * expr.t) =>
+      let (name, e) := mem in
+      let id := idexpr_id scope_none name in
+      expr_binop binop.eq (expr_id id) (expr_memdot (expr_id (idexpr_id scope_none "other")) id))
+      members in
+  let all_member_eq := fold_right
+    (fun (x y : expr_t) => expr_binop binop.logic_and x y)
+    (expr_id (idexpr_id scope_none "true")) member_compare in
+  let specialized_eq_operator :=
+    decl_fundef
+      declspec.none
+      (funtypeexpr_make
+        (typeexpr_primitive primtype.bool)
+        (make_funargs (funarg_named (cg.constref_of repr_cls_type) "other" :: nil))
+        (fnqual.set_noexcept (fnqual.set_const fnqual.none))
+        false)
+      (idexpr_operator scope_none (overloadable_operator.binary binop.eq))
+      attrspec.none
+      (funbody_stmts cinits_nil
+        (make_stmts (stmt_return all_member_eq :: nil))) in
+  decl_class
+    repr_cls_id
     true
-    (clsinherits_cons (clsinherit false visibility_spec.vis_public (idexpr_id scope_none "repr_base")) clsinherits_nil)
-    (make_clsdecls 
+    (clsinherits_cons (clsinherit_single false visibility_spec.vis_public base_cls_id) clsinherits_nil)
+    (make_clsdecls
       ((clsdecl_group
         visibility_spec.vis_public
-        (make_decls (cls_constructor :: member_decls))) :: nil)).
+        (make_decls (cls_constructor :: specialized_eq_operator :: overridden_eq_operator :: member_decls))) :: nil)).
 
 (*
   Roughly builds the following:
@@ -274,17 +346,17 @@ Definition make_single_match_test
     : condition_t * stmt_t :=
   let target_type := cg.constptr_of as_type in
   let temp_expr := expr_id temp_name in
-  let callargs := 
-    map 
-      (fun member => 
+  let callargs :=
+    map
+      (fun member =>
         expr_memarrow (expr_id temp_name) (idexpr_id scope_none member))
       members in
   let cond := (condition_decl
-      nil (cg.type_auto) temp_name nil
+      declspec.none (cg.type_auto) temp_name attrspec.none
       (expr_dynamic_cast target_type base_expr)) in
-  let body := 
+  let body :=
     stmt_block (
-      make_stmts 
+      make_stmts
         ((stmt_return (expr_call call_expr (make_callargs callargs))) :: nil)) in
   (cond, body).
 
@@ -305,7 +377,7 @@ Fixpoint make_match_constructors
       let cons_members := constructor_reprclass_members cons in
       let member_names := map fst cons_members in
       let as_type := typeexpr_id (idexpr_id scope_none cons_name) in
-      let temp_name := idexpr_id scope_none "tmp" in 
+      let temp_name := idexpr_id scope_none "tmp" in
       let (cond, body) := make_single_match_test base_expr as_type temp_name call_expr member_names in
       stmt_ifelse cond body sub
   end.
@@ -336,9 +408,9 @@ Definition make_match_fntype
       (* the formal arguments of our "match" function *)
       let formal_args :=
         make_funargs (
-          map 
+          map
             (fun name =>
-             funarg_named 
+             funarg_named
               (cg.constref_of (cg.named_type ("F" ++ name)))
               ("f" ++ name))
             consnames) in
@@ -351,9 +423,9 @@ Definition make_match_fntype
         cg.declval_of (cg.constref_of type)) pre_callargs in
       let ret_type :=
         typeexpr_decltype (expr_call (expr_id (idexpr_id scope_none ("F" ++ (inductive_constructor.name first_constructor)))) (make_callargs callargs)) in
-      (tplargs, funtypeexpr ret_type formal_args true)
+      (tplargs, funtypeexpr_make ret_type formal_args fnqual.none true)
     | nil =>
-      (nil, funtypeexpr (typeexpr_primitive primtype.void) funargs_nil false)
+      (nil, funtypeexpr_make (typeexpr_primitive primtype.void) funargs_nil fnqual.none false)
   end.
 
 Definition make_inductive_cons_factory_fn
@@ -373,24 +445,28 @@ Definition make_inductive_cons_factory_fn
         cg.move_of (expr_id (idexpr_id scope_none name)))
       cons_args in
   let fntype :=
-    funtypeexpr 
-      (cg.named_type ind_clsname) 
+    funtypeexpr_make
+      (cg.named_type ind_clsname)
       (make_funargs formal_args)
+      fnqual.none
       false in
-  let repr_instance := 
-    cg.make_shared_of 
-      (cg.named_type (consname ++ "_repr")) 
+  let repr_instance :=
+    cg.make_shared_of
+      (cg.named_type (consname ++ "_repr"))
       args in
   let cls_instance :=
     expr_call (expr_id (idexpr_id scope_none ind_clsname)) (make_callargs (repr_instance :: nil)) in
   decl_fundef
-    (decl_specifier.ds_static :: nil)
+    (declspec.set_static declspec.none)
     fntype
     (idexpr_id scope_none consname)
-    nil
-    (make_stmts (stmt_return cls_instance :: nil)).
+    attrspec.none
+    (funbody_stmts
+      cinits_nil
+      (make_stmts (stmt_return cls_instance :: nil))).
 
-Definition one_inductive_decl (oi : one_inductive.t) : decl_t :=
+Definition one_inductive_decl_parts (oi : one_inductive.t)
+    : tplformargs_t * idexpr_t * clsdecls_t :=
   let environ := env.empty in
   let (name, sig, constructors) := oi in
 
@@ -419,15 +495,18 @@ Definition one_inductive_decl (oi : one_inductive.t) : decl_t :=
   (* match function to discriminate between the different constructors *)
   let (match_fn_tplargs, match_fn_type) := make_match_fntype constructors environ in
   let cons_call := map
-    (fun (cons : inductive_constructor.t) => 
+    (fun (cons : inductive_constructor.t) =>
       (cons, expr_id (idexpr_id scope_none ("f" ++ inductive_constructor.name cons)))) constructors in
-  let match_fn_decl := 
-    decl_fundef 
-      nil 
+  let match_fn_decl :=
+    decl_fundef
+      declspec.none
       match_fn_type
-      (idexpr_id scope_none "match") 
-      nil 
-      (stmts_cons (make_match_constructors (expr_id id_repr_m) cons_call) stmts_nil) in
+      (idexpr_id scope_none "match")
+      attrspec.none
+      (funbody_stmts
+        cinits_nil
+        (make_stmts
+          (make_match_constructors (expr_id id_repr_m) cons_call :: nil))) in
   let match_fn_tpldecl := maybe_template (make_tplformargs match_fn_tplargs) match_fn_decl in
 
   (* The static factory functions to create instances of this object
@@ -444,61 +523,90 @@ Definition one_inductive_decl (oi : one_inductive.t) : decl_t :=
   (* C++ class constructors *)
   let primary_constructor :=
     decl_consdesdef
-      (decl_specifier.ds_explicit :: nil)
+      (declspec.set_explicit declspec.none)
       cls_id
       (make_funargs ((funarg_named repr_ptr_type "repr") :: nil))
-      (attr_specifier.as_noexcept :: nil)
-      (ctor_initializers_cons (ctor_initializer (idexpr_id scope_none "repr_") (cg.move_of (expr_id (idexpr_id scope_none "repr")))) ctor_initializers_nil)
-      (make_stmts nil) in
+      (fnqual.set_noexcept fnqual.none)
+      attrspec.none
+      (funbody_stmts
+        (cinits_cons (cinit_make (idexpr_id scope_none "repr_") (cg.move_of (expr_id (idexpr_id scope_none "repr")))) cinits_nil)
+        (make_stmts nil)) in
   let copy_constructor :=
-    decl_consdesdef_special
-      nil
+    decl_consdesdef
+      declspec.none
       cls_id
       (make_funargs (((funarg_named (cg.constref_of cls_type) "other")) :: nil))
-      (attr_specifier.as_noexcept :: nil)
-      special_fundef.def_default in
+      (fnqual.set_noexcept fnqual.none)
+      attrspec.none
+      funbody_default in
   let move_constructor :=
-    decl_consdesdef_special
-      nil
+    decl_consdesdef
+      declspec.none
       cls_id
       (make_funargs (((funarg_named (typeexpr_rvaluereference cls_type) "other")) :: nil))
-      (attr_specifier.as_noexcept :: nil)
-      special_fundef.def_default in
+      (fnqual.set_noexcept fnqual.none)
+      attrspec.none
+      funbody_default in
   let default_constructor := cg.deleted_constructor cls_name nil in
 
   let assign_operator :=
     decl_fundef
-      nil
-      (funtypeexpr
+      declspec.none
+      (funtypeexpr_make
         (typeexpr_reference cls_type)
         (make_funargs (funarg_named (cg.constref_of cls_type) "other" :: nil))
+        (fnqual.set_noexcept fnqual.none)
         false)
       (idexpr_operator scope_none (overloadable_operator.binary binop.assign))
-      (attr_specifier.as_noexcept :: nil)
-      (make_stmts (
-        stmt_expr (expr_binop binop.assign (expr_id id_repr_m)
-          (expr_memarrow (expr_id (idexpr_id scope_none "other")) id_repr_m)) ::
-        stmt_return (expr_unop unop.deref (expr_id (idexpr_id scope_none "this"))) ::
-        nil)) in
+      attrspec.none
+      (funbody_stmts
+        cinits_nil
+        (make_stmts (
+          stmt_expr (expr_binop binop.assign (expr_id id_repr_m)
+            (expr_memarrow (expr_id (idexpr_id scope_none "other")) id_repr_m)) ::
+          stmt_return (expr_unop unop.deref (expr_id (idexpr_id scope_none "this"))) ::
+          nil))) in
 
   let assign_move_operator :=
     decl_fundef
-      nil
-      (funtypeexpr
+      declspec.none
+      (funtypeexpr_make
         (typeexpr_reference cls_type)
         (make_funargs (funarg_named (typeexpr_rvaluereference cls_type) "other" :: nil))
+        (fnqual.set_noexcept fnqual.none)
         false)
       (idexpr_operator scope_none (overloadable_operator.binary binop.assign))
-      (attr_specifier.as_noexcept :: nil)
-      (make_stmts (
-        stmt_expr (expr_binop binop.assign (expr_id id_repr_m)
-          (cg.move_of (expr_memarrow (expr_id (idexpr_id scope_none "other")) id_repr_m))) ::
-        stmt_return (expr_unop unop.deref (expr_id (idexpr_id scope_none "this"))) ::
-        nil)) in
+      attrspec.none
+      (funbody_stmts
+        cinits_nil
+        (make_stmts (
+          stmt_expr (expr_binop binop.assign (expr_id id_repr_m)
+            (cg.move_of (expr_memarrow (expr_id (idexpr_id scope_none "other")) id_repr_m))) ::
+          stmt_return (expr_unop unop.deref (expr_id (idexpr_id scope_none "this"))) ::
+          nil))) in
 
-  let repr_member_decl := (decl_simple nil repr_ptr_type id_repr_m nil) in
-  let d := decl_class cls_id false clsinherits_nil
-    (make_clsdecls 
+  let eq_operator :=
+    decl_fundef
+      declspec.none
+      (funtypeexpr_make
+        (typeexpr_primitive primtype.bool)
+        (make_funargs (funarg_named (cg.constref_of cls_type) "other" :: nil))
+        (fnqual.set_noexcept (fnqual.set_const fnqual.none))
+        false)
+      (idexpr_operator scope_none (overloadable_operator.binary binop.eq))
+      attrspec.none
+      (funbody_stmts cinits_nil
+        (make_stmts
+          (stmt_return
+            (expr_binop binop.eq
+              (expr_unop unop.deref (expr_id id_repr_m))
+              (expr_unop unop.deref (expr_memdot
+                (expr_id (idexpr_id scope_none "other")) id_repr_m))) ::
+          nil))) in
+
+  let repr_member_decl := (decl_simple declspec.none repr_ptr_type id_repr_m attrspec.none) in
+  let clsdecls :=
+    (make_clsdecls
       ((clsdecl_group
         visibility_spec.vis_public
         (make_decls
@@ -507,25 +615,230 @@ Definition one_inductive_decl (oi : one_inductive.t) : decl_t :=
            move_constructor ::
            assign_operator ::
            assign_move_operator ::
+           eq_operator ::
            factory_fns ++
-           match_fn_tpldecl :: 
+           match_fn_tpldecl ::
            nil))) ::
       (clsdecl_group
         visibility_spec.vis_private
         (make_decls (
           repr_base_class_def ::
-          repr_classes ++ 
-          primary_constructor :: 
-          repr_member_decl :: 
+          repr_classes ++
+          primary_constructor ::
+          repr_member_decl ::
           nil))) ::
       nil)) in
-  maybe_template tpl d.
+  (tpl, cls_id, clsdecls).
 
-Fixpoint to_decls (l : list decl_t) :=
-  match l with
-    | nil => decls_nil
-    | cons d l => decls_cons d (to_decls l)
+Definition one_inductive_decl (oi : one_inductive.t) : decl_t :=
+  let (x, clsdecls) := one_inductive_decl_parts oi in
+  let (tplargs, cls_id) := x in
+  maybe_template tplargs (decl_class cls_id true clsinherits_nil clsdecls).
+
+(* If a decl_t is actually a definition of something, turn this into
+a (forward) declaration of the object. This can be either variables,
+functions or classes. *)
+Fixpoint decl_remove_def (decl : decl_t) : decl_t :=
+  match decl with
+    | decl_initdef ds type id attrs value =>
+      decl_simple ds type id attrs
+    | decl_fundef ds funtype id attrs body =>
+      if funbody_is_stmts body then
+        decl_simple ds (typeexpr_function funtype) id attrs
+      else
+        decl
+    | decl_consdesdef ds id args qual attrs body =>
+      if funbody_is_stmts body then
+        decl_consdesdecl ds id args qual attrs
+      else
+        decl
+    | decl_class id is_final inherits decls =>
+      decl_class_fwd id
+    | decl_templated args decl =>
+      decl_templated args (decl_remove_def decl)
+    | _ => decl
   end.
+
+Fixpoint decls_remove_defs (decls : decls_t) : decls_t :=
+  match decls with
+    | decls_nil => decls_nil
+    | decls_cons decl decls =>
+      decls_cons (decl_remove_def decl) (decls_remove_defs decls)
+  end.
+
+Fixpoint clsdecls_remove_defs (cdecls : clsdecls_t) : clsdecls_t :=
+  match cdecls with
+    | clsdecls_nil => clsdecls_nil
+    | clsdecls_cons cdecl cdecls =>
+      let (vis, decls) := cdecl in
+      let decls := decls_remove_defs decls in
+      let cdecl := clsdecl_group vis decls in
+      clsdecls_cons cdecl (clsdecls_remove_defs cdecls)
+  end.
+
+Fixpoint cls_remove_defs (decl : decl_t) : decl_t :=
+  match decl with
+    | decl_class id is_final inherits clsdecls =>
+      decl_class id is_final inherits (clsdecls_remove_defs clsdecls)
+    | decl_templated args decl =>
+      decl_templated args (cls_remove_defs decl)
+    | _ => decl
+  end.
+
+Fixpoint scope_concat (s1 s2 : scope_t) : scope_t :=
+  match s1 with
+    | scope_none => s2
+    | scope_id id s => scope_id id (scope_concat s s2)
+    | scope_template tplid s => scope_template tplid (scope_concat s s2)
+  end.
+
+Definition idexpr_nest_scope (scope : scope_t) (e : idexpr_t) :=
+  match e with
+    | idexpr_id s id => idexpr_id (scope_concat scope s) id
+    | idexpr_destructor s id => idexpr_destructor (scope_concat scope s) id
+    | idexpr_template s tplid => idexpr_template (scope_concat scope s) tplid
+    | idexpr_operator s op => idexpr_operator (scope_concat scope s) op
+  end.
+
+Fixpoint decl_scopify (scope : scope_t) (decl : decl_t) :=
+  match decl with
+    | decl_simple ds type id attr =>
+      decl_simple ds type (idexpr_nest_scope scope id) attr
+    | decl_initdef ds type id attr value =>
+      decl_initdef ds type (idexpr_nest_scope scope id) attr value
+    | decl_fundef ds funtype id attr body =>
+      decl_fundef ds funtype (idexpr_nest_scope scope id) attr body
+    | decl_consdesdecl ds id args qual attr =>
+      decl_consdesdecl ds (idexpr_nest_scope scope id) args qual attr
+    | decl_consdesdef ds id args qual attr body =>
+      decl_consdesdef ds (idexpr_nest_scope scope id) args qual attr body
+    | decl_class_fwd id =>
+      decl_class_fwd (idexpr_nest_scope scope id)
+    | decl_class id is_final inherits clsdecls =>
+      decl_class (idexpr_nest_scope scope id) is_final inherits clsdecls
+    | decl_templated formargs decl =>
+      decl_templated formargs (decl_scopify scope decl)
+  end.
+
+(* Clear decl specifiers that may be applied to a class member but
+that have a different meaning / are illegal when un-inlining the definition
+of the class member *)
+Definition declspec_extract_member (ds : declspec.t) : declspec.t :=
+  let ds := declspec.clear_static ds in
+  let ds := declspec.clear_mutable ds in
+  let ds := declspec.clear_virtual ds in
+  let ds := declspec.clear_explicit ds in
+  let ds := declspec.clear_friend ds in
+  ds.
+
+Definition attrspec_extract_member (attr : attrspec.t) : attrspec.t :=
+  attrspec.none.
+
+Fixpoint decl_is_member_def (decl : decl_t) : bool :=
+  match decl with
+    | decl_simple ds type id attr =>
+      false
+    | decl_initdef ds type id attr value =>
+      declspec.is_static ds
+    | decl_fundef ds funtype id attr body =>
+      funbody_is_stmts body
+    | decl_consdesdecl ds id args qual attr =>
+      false
+    | decl_consdesdef ds id args qual attr body =>
+      funbody_is_stmts body
+    | decl_class_fwd id =>
+      false
+    | decl_class id is_final inherits clsdecls =>
+      true
+    | decl_templated formargs decl =>
+      decl_is_member_def decl
+  end.
+
+Fixpoint decl_extract_member_def (decl : decl_t) : decl_t :=
+  match decl with
+    | decl_initdef ds type id attr value =>
+      decl_initdef (declspec_extract_member ds) type id (attrspec_extract_member attr) value
+    | decl_fundef ds funtype id attr body =>
+      decl_fundef (declspec_extract_member ds) funtype id (attrspec_extract_member attr) body
+    | decl_consdesdef ds id args qual attr body =>
+      decl_consdesdef (declspec_extract_member ds) id args qual (attrspec_extract_member attr) body
+    | decl_class id is_final inherits clsdecls =>
+      decl_class id is_final inherits clsdecls
+    | decl_templated formargs decl =>
+      decl_templated formargs (decl_extract_member_def decl)
+    | _ => decl
+  end.
+
+Fixpoint decls_extract_member_defs (decls : decls_t) : list decl_t :=
+  match decls with
+    | decls_nil => nil
+    | decls_cons decl decls =>
+      (if decl_is_member_def decl then
+        (decl_extract_member_def decl) :: nil
+      else
+        nil) ++ decls_extract_member_defs decls
+  end.
+
+Definition clsdecl_extract_member_defs (clsdecl : clsdecl_t) : list decl_t :=
+  let (visibility, decls) := clsdecl in
+  decls_extract_member_defs decls.
+
+Fixpoint clsdecls_extract_member_defs (clsdecls : clsdecls_t) : list decl_t :=
+  match clsdecls with
+    | clsdecls_nil => nil
+    | clsdecls_cons clsdecl clsdecls =>
+      (clsdecl_extract_member_defs clsdecl) ++ (clsdecls_extract_member_defs clsdecls)
+  end.
+
+Definition idexpr_maybe_template (tplargs : tplargs_t) (id : idexpr_t) : idexpr_t :=
+  match id with
+    | idexpr_id scope id =>
+      idexpr_template scope (templateid_make id tplargs)
+    | idexpr_destructor scope _ =>
+      id (* illegal *)
+    | idexpr_template scope tplid =>
+      let (id, tplargs2) := tplid in
+      idexpr_template scope (templateid_make id tplargs) (* XXX: concat tplargs *)
+    | idexpr_operator scope op =>
+      id
+  end.
+
+Definition idexpr_to_scope (idexpr : idexpr_t) : scope_t :=
+  match idexpr with
+    | idexpr_id scope id =>
+      scope_concat scope (scope_id id scope_none)
+    | idexpr_destructor scope id =>
+      scope (* illegal *)
+    | idexpr_template scope tplid =>
+      scope_concat scope (scope_template tplid scope_none)
+    | idexpr_operator scope op =>
+      scope (* illegal *)
+  end.
+
+Definition generate_member_defs
+    (tplargs : tplformargs_t) (id : idexpr_t) (decls : clsdecls_t)
+    : list decl_t :=
+  let clsid := idexpr_maybe_template (tplformargs_to_tplargs tplargs) id in
+  let scope := idexpr_to_scope clsid in
+  let edecls := (clsdecls_extract_member_defs decls) in
+  let replace_id_fn :=
+    (fun (o : idexpr_t) =>
+      match o with
+        | idexpr_id scope_none o_id =>
+          match id with
+            | idexpr_id scope_none i_id =>
+              if string_dec o_id i_id then clsid else o
+            | _ => o
+          end
+        | _ => o
+      end) in
+  let edecls := map (decl_replace_idexpr replace_id_fn) edecls in
+  map (maybe_template tplargs) (map (decl_scopify scope) edecls).
+
+Definition generate_stripped_class_def
+    (tplargs : tplformargs_t) (id : idexpr_t) (decls : clsdecls_t)
+    : decl_t :=
+  (maybe_template tplargs (decl_class id true clsinherits_nil (clsdecls_remove_defs decls))).
 
 Example sort_set := (expr.global "Set"%string).
 
@@ -542,21 +855,30 @@ Example oiX :=
         (expr.app (expr.global "X"%string) (expr.local "T"%string 1))) ::
     nil).
 
+
 Example i1 := inductive.make (oiX :: nil).
 
 Eval lazy in (collect_tplformargs_from_product (let (_, sig, _) := oiX in sig)).
 
-Eval lazy in (serialize_tokens (decls_serialize (to_decls (inductive_fwd i1)))).
+Eval lazy in (serialize_tokens (decls_serialize (make_decls (inductive_fwd i1)))).
 
 Eval lazy in (serialize_tokens (decl_serialize (one_inductive_decl oiX))).
 
+Eval lazy in (serialize_tokens (decl_serialize (cls_remove_defs (one_inductive_decl oiX)))).
+
+Example icls1 := one_inductive_decl_parts oiX.
+
+Example icls1_tplargs := fst (fst icls1).
+Example icls1_idexpr := snd (fst icls1).
+Example icls1_cdecls := snd icls1.
+
+Eval lazy in (serialize_tokens (decl_serialize (generate_stripped_class_def icls1_tplargs icls1_idexpr icls1_cdecls))).
+Eval lazy in (serialize_tokens (decls_serialize (make_decls (generate_member_defs icls1_tplargs icls1_idexpr icls1_cdecls)))).
 
 (*
 
 TODO:
 
-- equality operator of X ???
-- un-inline from declaration
 - full support for mutual inductive defs
 
 DONE:
@@ -564,6 +886,8 @@ DONE:
 + C++ constructors of X
 + C++ factory functions corresponding to inductive constructors
 + C++ constructors of repr classes
-- assignment operator of X
++ equality operator of X
++ assignment operator of X
++ un-inline from declaration
 
 *)
